module proofs where

open import lib

sym : ∀{i}{A : Set i}{x y : A} → x ≡ y → y ≡ x
sym refl = refl

trans : ∀{i}{A : Set i}{x y z : A} → x ≡ y → y ≡ z → x ≡ z
trans refl eq2 = eq2

cong : ∀{i j}{A : Set i}{B : Set j}(f : A → B){x y : A} → x ≡ y → f x ≡ f y
cong f refl = refl

cong₂ : ∀{i j k}{A : Set i}{B : Set j}{C : Set k}(f : A → B → C){x x' : A}{y y' : B} →
  x ≡ x' → y ≡ y' → f x y ≡ f x' y'
cong₂ f refl refl = refl

cong₃ : ∀{i j k l}{A : Set i}{B : Set j}{C : Set k}{D : Set l}(f : A → B → C → D){x x' : A}{y y' : B}{z z' : C} →
  x ≡ x' → y ≡ y' → z ≡ z' → f x y z ≡ f x' y' z'
cong₃ f refl refl refl = refl

subst : ∀{i j}{A : Set i}(P : A → Set j){x y : A} → x ≡ y → P x → P y
subst P refl px = px

_≡⟨_⟩_ : ∀{i}{A : Set i}(x : A){y z : A} → x ≡ y → y ≡ z → x ≡ z
_ ≡⟨ p ⟩ q = trans p q

_∎ : ∀{i}{A : Set i}(x : A) → x ≡ x
_ ∎ = refl

infixr 2 _≡⟨_⟩_
infix 3 _∎

idr+ : (n : ℕ) → n + zero ≡ n
idr+ zero = refl
idr+ (suc n) = cong suc (idr+ n)

sucr+ : (n m : ℕ) → n + suc m ≡ suc (n + m)
sucr+ zero m = refl
sucr+ (suc n) m = cong (λ x → suc x) (sucr+ n m)

ass+ : (m n o : ℕ) → (m + n) + o ≡ m + (n + o)
ass+ zero n o = refl
ass+ (suc m) n o = cong suc (ass+ m n o)

comm+ : (m n : ℕ) → m + n ≡ n + m
comm+ zero n = sym (idr+ n)
comm+ (suc m) n = trans (cong suc (comm+ m n)) (sym (sucr+ n m))

dist+* : (m n o : ℕ) → (m + n) * o ≡ m * o + n * o
dist+* zero n o = refl
dist+* (suc m) n o = trans (cong (o +_) (dist+* m n o)) (sym (ass+ o (m * o) (n * o)))

dist*+ : (m n o : ℕ) → m * (n + o) ≡ m * n + m * o
dist*+ zero n o = refl
dist*+ (suc m) n o =
  n + o + m * (n + o)
  ≡⟨ ass+ n o (m * (n + o)) ⟩
  n + (o + m * (n + o)) 
  ≡⟨ cong (n +_) (comm+ o (m * (n + o))) ⟩
  n + (m * (n + o) + o)
  ≡⟨ sym (ass+ n (m * (n + o)) o) ⟩
  n + m * (n + o) + o
  ≡⟨ cong (λ x → n + x + o) (dist*+ m n o) ⟩
  n + (m * n + m * o) + o
  ≡⟨ cong (_+ o) (sym (ass+ n (m * n) (m * o))) ⟩
  n + m * n + m * o + o
  ≡⟨ ass+ (n + m * n) (m * o) o ⟩
  n + m * n + (m * o + o)
  ≡⟨ cong ((n + m * n) +_) (comm+ (m * o) o) ⟩
  n + m * n + (o + m * o) ∎

nullr* : (n : ℕ) → n * 0 ≡ 0
nullr* zero = refl
nullr* (suc n) = nullr* n

idl* : (n : ℕ) → 1 * n ≡ n
idl* = idr+ 

idr* : (n : ℕ) → n * 1 ≡ n
idr* zero = refl
idr* (suc n) = cong suc (idr* n)

sucr* : (n m : ℕ) → n * suc m ≡ n + n * m
sucr* zero m = refl
sucr* (suc n) m =
  suc (m + n * suc m)
  ≡⟨ cong suc (comm+ m (n * suc m)) ⟩
  suc (n * suc m + m)
  ≡⟨ cong (λ x → suc (x + m)) (sucr* n m) ⟩
  suc (n + n * m + m)
  ≡⟨ cong suc (ass+ n (n * m) m) ⟩
  suc (n + (n * m + m))
  ≡⟨ cong (λ x → suc (n + x)) (comm+ (n * m) m) ⟩
  suc (n + (m + n * m)) ∎

ass* : (m n o : ℕ) → (m * n) * o ≡ m * (n * o)
ass* zero n o = refl
ass* (suc m) n o =
  (n + m * n) * o
  ≡⟨ dist+* n (m * n) o ⟩
  n * o + m * n * o 
  ≡⟨ cong (n * o +_) (ass* m n o) ⟩
  n * o + m * (n * o) ∎

comm* : (m n : ℕ) → m * n ≡ n * m
comm* zero n = sym (nullr* n)
comm* (suc m) n =
  n + m * n
  ≡⟨ cong (n +_) (comm* m n) ⟩
  n + n * m
  ≡⟨ sym (sucr* n m) ⟩
  n * suc m ∎

sucinj : ∀{x y} → suc x ≡ suc y → x ≡ y
sucinj refl = refl